Splinter/Betree/BufferOffsets.i.dfy
@@ -21,13 +21,6 @@ module BufferOffsetsMod
       offsets[i]
     }
 
-    // todo(tony): Duplicate with AdvanceIndex
-    // function Update(i: nat, v:nat): BufferOffsets 
-    //   requires i < |offsets|
-    // {
-    //   BufferOffsets(offsets[i := v])
-    // }
-
     predicate BoundedBy(length: nat)
       ensures BoundedBy(length) == forall i:nat | i < |offsets| :: Get(i) <= length
     {
