Splinter/Betree/OffsetMap.i.dfy
@@ -1,0 +1,50 @@
+// Copyright 2018-2021 VMware, Inc., Microsoft Inc., Carnegie Mellon University, ETH Zurich, and University of Washington
+// SPDX-License-Identifier: BSD-2-Clause
+
+include "../../lib/Base/KeyType.s.dfy"
+include "Buffer.i.dfy"
+
+
+module OffsetMapMod {
+  import opened KeyType
+  import opened BufferMod
+
+
+  // TotalMapMod provides something like these, but it depends on module
+  // refinement that's hairy and has problems in use (rank_is_less_than doesn't
+  // make it through the module refinement, so we can't prove decreases).
+  predicate AnyKey(key: Key) { true }
+  predicate Total(keys: iset<Key>) {
+    forall k | AnyKey(k) :: k in keys
+  }
+  function AllKeys() : (out: iset<Key>)
+    ensures Total(out)
+  {
+    iset k | AnyKey(k)
+  }
+
+  datatype OffsetMap = OffsetMap(offsets: imap<Key, nat>)
+  {
+    predicate WF() {
+      Total(offsets.Keys)
+    }
+
+    function Get(k: Key) : nat 
+      requires WF()
+    {
+      offsets[k]
+    }
+
+    function FilterForBottom() : iset<Key> 
+      requires WF()
+    {
+      iset k | offsets[k] == 0
+    }
+
+    function Decrement(i: nat) : OffsetMap 
+      requires WF()
+    {
+      OffsetMap(imap k | AnyKey(k) :: if i <= offsets[k] then offsets[k]-i else 0)
+    }
+  }
+}
