Splinter/Betree/PagedBetree.i.dfy
@@ -29,6 +29,7 @@ module PagedBetree
   import opened LSNMod
   import opened Sequences
   import opened BufferMod
+  import opened OffsetMapMod
   import opened BufferStackMod
   import opened MemtableMod
 
